Added transitivity as lemma

language_formalisation/type_system/subtyping.v
@@ -1,11 +1,10 @@
 Add LoadPath "C:\Users\Ziga\Documents\Ziga_podatki\PHD\language_formalisation\syntax".
-Require Import syntax Relation_Definitions.
+Require Import syntax.
 
 
 Inductive vsubtype : vtype -> vtype -> Prop :=
-| VsubtyRefl A : vsubtype A A
-| VsubtyTrans A1 A2 A3: vsubtype A1 A2 -> vsubtype A2 A3 -> vsubtype A1 A3
-| VsubtyStruc A B : vsubtype A B -> vsubtype A B
+| VsubtyUnit : vsubtype TyUnit TyUnit
+| VsubtyInt : vsubtype TyInt TyInt
 | VsubtyTyΣ A A' B B' : 
     vsubtype A A' -> vsubtype B B' -> vsubtype (TyΣ A B) (TyΣ A' B')
 | VsubtyTyΠ A A' B B' : 
@@ -26,33 +25,77 @@ with sigsubtype : sig -> sig -> Prop :=
     -> sigsubtype Σ Σ'
 .
 
+Ltac inv H := inversion H; clear H; subst.
 
-
-
-(*
-Inductive vsubtype : vtype -> vtype -> Prop :=
-| VsubtyRefl A : vsubtype A A
-| VsubtyTrans A1 A2 A3 : vsubtype A1 A2 -> vsubtype A2 A3 -> vsubtype A1 A3
-| VsubtyTyΣ A A' B B' : 
-    vsubtype A A' -> vsubtype B B' -> vsubtype (TyΣ A B) (TyΣ A' B')
-| VsubtyTyΠ A A' B B' : 
-    vsubtype A A' -> vsubtype B B' -> vsubtype (TyΠ A B) (TyΠ A' B')
-| VsubtyFun A A' C C' : 
-    vsubtype A' A -> csubtype C C' -> vsubtype (TyFun A C) (TyFun A' C')
-| VsubtyHandler C C' D D': 
-    csubtype C' C -> csubtype D D' -> vsubtype (TyHandler C D) (TyHandler C' D')
-
-with csubtype : ctype -> ctype -> Prop  :=
-| CsubtyRefl C : csubtype C C
-| CsubtyTrans C1 C2 C3 : csubtype C1 C2 -> csubtype C2 C3 -> csubtype C1 C3
-| Csubty A A' Σ Σ' E : 
-    vsubtype A A' -> sigsubtype Σ Σ' -> csubtype (CTy A Σ E) (CTy A' Σ' E)
-
-with sigsubtype : sig -> sig -> Prop :=
-| ΣsubtyRefl Σ : sigsubtype Σ Σ
-| ΣsubtyTrans Σ1 Σ2 Σ3 : sigsubtype Σ1 Σ2 -> sigsubtype Σ2 Σ3 -> sigsubtype Σ1 Σ3
-| Σsubty Σ Σ':
-    (forall op A B A' B', (get_op_type Σ op = Some (A, B) -> 
-      (get_op_type Σ' op = Some (A', B')) /\ vsubtype A' A /\ vsubtype B B'))
-    -> sigsubtype Σ Σ'
-. *)
+(* Weird notation for SPEED! *)
+Fixpoint vsubtype_trans A1 A2 A3 
+  (A12 : vsubtype A1 A2) {struct A12} : vsubtype A2 A3 -> vsubtype A1 A3
+with vsubtype_trans_rev A1 A2 A3
+  (A21 : vsubtype A2 A1) {struct A21} : vsubtype A3 A2 -> vsubtype A3 A1
+with csubtype_trans C1 C2 C3
+  (C12 : csubtype C1 C2) {struct C12} : csubtype C2 C3 -> csubtype C1 C3
+with csubtype_trans_rev C1 C2 C3 
+  (C21 : csubtype C2 C1) {struct C21} : csubtype C3 C2 -> csubtype C3 C1
+with sigsubtype_trans Σ1 Σ2 Σ3 
+  (S12 : sigsubtype Σ1 Σ2) {struct S12} : sigsubtype Σ2 Σ3 -> sigsubtype Σ1 Σ3
+with sigsubtype_trans_rev Σ1 Σ2 Σ3
+  (S21 : sigsubtype Σ2 Σ1) {struct S21} : sigsubtype Σ3 Σ2-> sigsubtype Σ3 Σ1.
+Proof.
+{
+clear sigsubtype_trans sigsubtype_trans_rev.
+intros A23; destruct A12; try assumption; inv A23.
++ apply VsubtyTyΣ.
+  - eapply vsubtype_trans. exact A12_1. assumption.
+  - eapply vsubtype_trans. exact A12_2. assumption.
++ apply VsubtyTyΠ.
+  - eapply vsubtype_trans. exact A12_1. assumption.
+  - eapply vsubtype_trans. exact A12_2. assumption.
++ apply VsubtyFun.
+  - eapply vsubtype_trans_rev. exact A12. assumption. 
+  - eapply csubtype_trans. exact H. assumption.
++ apply VsubtyHandler.
+  - eapply csubtype_trans_rev. exact H. assumption. 
+  - eapply csubtype_trans. exact H0. assumption.
+}{
+clear sigsubtype_trans sigsubtype_trans_rev.
+intros A32; destruct A21; try assumption; inv A32.
++ apply VsubtyTyΣ.
+  - eapply vsubtype_trans_rev. exact A21_1. assumption.
+  - eapply vsubtype_trans_rev. exact A21_2. assumption.
++ apply VsubtyTyΠ.
+  - eapply vsubtype_trans_rev. exact A21_1. assumption.
+  - eapply vsubtype_trans_rev. exact A21_2. assumption.
++ apply VsubtyFun.
+  - eapply vsubtype_trans. exact A21. assumption. 
+  - eapply csubtype_trans_rev. exact H. assumption.
++ apply VsubtyHandler.
+  - eapply csubtype_trans. exact H. assumption. 
+  - eapply csubtype_trans_rev. exact H0. assumption.
+}{
+clear vsubtype_trans_rev csubtype_trans csubtype_trans_rev sigsubtype_trans_rev.
+intros C23; destruct C12. inv C23.
+apply Csubty.
+- eapply vsubtype_trans. exact H. assumption.
+- eapply sigsubtype_trans. exact H0. assumption.
+}{
+clear vsubtype_trans csubtype_trans csubtype_trans_rev sigsubtype_trans.
+intros C32; destruct C21. inv C32.
+apply Csubty.
+- eapply vsubtype_trans_rev. exact H. assumption.
+- eapply sigsubtype_trans_rev. exact H0. assumption.
+}{
+clear vsubtype_trans vsubtype_trans_rev.
+clear csubtype_trans csubtype_trans_rev.
+clear sigsubtype_trans sigsubtype_trans_rev.
+intros S23; destruct S12. inv S23.
+apply Σsubty. intros.
+apply H0. eapply H in H1. destruct H1. exact H1.
+}{
+clear vsubtype_trans vsubtype_trans_rev.
+clear csubtype_trans csubtype_trans_rev.
+clear sigsubtype_trans sigsubtype_trans_rev.
+intros S32; destruct S21. inv S32.
+apply Σsubty. intros.
+apply H. eapply H0 in H1. destruct H1. exact H1.
+}
+Qed.
