language_formalisation/type_system/subtyping_lemmas.v
@@ -1,0 +1,32 @@
+Add LoadPath "C:\Users\Ziga\Documents\Ziga_podatki\PHD\language_formalisation\syntax".
+Add LoadPath "C:\Users\Ziga\Documents\Ziga_podatki\PHD\language_formalisation\type_system".
+Require Import syntax declarational.
+
+
+Fixpoint subty_pi A B C :
+  vsubtype C (TyΠ A B) -> 
+  exists A' B', C = (TyΠ A' B') /\ vsubtype A' A /\ vsubtype B' B.
+Proof.
+intro orig.
+inv orig. exists A0. exists B0.
+constructor. reflexivity. constructor; assumption.
+Qed.
+
+
+Fixpoint subty_pair Γ v1 v2 A B :
+has_vtype Γ (Pair v1 v2) (TyΠ A B) ->
+has_vtype Γ v1 A /\ has_vtype Γ v2 B.
+Proof.
+intro orig. inv orig. inv H1. constructor; assumption.
+induction H3.
+
+
+intro orig. inv orig. inv H1. constructor; assumption.
+apply subty_pi in H3. destruct H3. destruct H1. destruct H1.
+subst. apply subty_pair in H2.
+destruct H2. destruct H3. constructor.
+- apply TypeV. assumption. inv H0. assumption.
+  eapply TypeVSubtype. exact H1. assumption.
+- apply TypeV. assumption. inv H0. assumption.
+  eapply TypeVSubtype. exact H2. assumption.
+Qed.
